src/TrsInv.v
@@ -4,27 +4,57 @@ Require Import Simulation Serial.
 
 Set Implicit Arguments.
 
+Definition Inv := TState -> Prop.
+
+Definition invAnd (inv1 inv2: Inv) :=
+  fun tst => inv1 tst /\ inv2 tst.
+Infix "/\i" := invAnd (at level 80).
+
+Definition invImp (inv1 inv2: Inv) :=
+  forall tst, inv1 tst -> inv2 tst.
+Infix "->i" := invImp (at level 99).
+
+Lemma inv_proj1: forall inv1 inv2, inv1 /\i inv2 ->i inv1.
+Proof. firstorder. Qed.
+Lemma inv_proj2: forall inv1 inv2, inv1 /\i inv2 ->i inv2.
+Proof. firstorder. Qed.
+
+Definition AInv := TInfo -> History -> MessagePool TMsg -> TState -> Prop.
+Definition ainvAnd (ainv1 ainv2: AInv) :=
+  fun ti hst mouts tst =>
+    ainv1 ti hst mouts tst /\ ainv2 ti hst mouts tst.
+Infix "/\a" := ainvAnd (at level 80).
+Definition ainvImp (ainv1 ainv2: AInv) :=
+  forall ti hst mouts tst,
+    ainv1 ti hst mouts tst -> ainv2 ti hst mouts tst.
+Infix "->a" := ainvImp (at level 99).
+
+Lemma ainv_proj1: forall ainv1 ainv2, ainv1 /\a ainv2 ->a ainv1.
+Proof. firstorder. Qed.
+Lemma ainv_proj2: forall ainv1 ainv2, ainv1 /\a ainv2 ->a ainv2.
+Proof. firstorder. Qed.
+
 Section Impl.
   Variable (impl: System).
 
-  Definition TrsInvInit (ginv: TState -> Prop) :=
+  Definition TrsInvInit (ginv: Inv) :=
     ginv (getStateInit impl).
 
-  Definition TrsInv (ginv: TState -> Prop) :=
+  Definition TrsInv (ginv: Inv) :=
     forall ist1,
       ginv ist1 ->
       forall ihst ist2,
         trsSteps impl ist1 ihst ist2 ->
         ginv ist2.
 
-  Definition TrsInvIn (ginv: TState -> Prop) :=
+  Definition TrsInvIn (ginv: Inv) :=
     forall ist1,
       ginv ist1 ->
       forall imin ist2,
         step_det impl ist1 (IlblIn imin) ist2 ->
         ginv ist2.
 
-  Definition TrsInvAtomic (ginv: TState -> Prop) :=
+  Definition TrsInvAtomic (ginv: Inv) :=
     forall ti hst mouts orsout,
       Atomic impl ti hst mouts orsout ->
       forall ist1,
@@ -33,12 +63,7 @@ Section Impl.
           steps_det impl ist1 hst ist2 ->
           ginv ist2.
 
-  Definition TrsAInvInit
-             (ainv: TInfo -> History -> MessagePool TMsg -> TState -> Prop) :=
-    forall ti tst, ainv ti nil (enqMP (toTMsgU (tinfo_rqin ti)) nil) tst.
-
-  Definition TrsAInv (ginv: TState -> Prop)
-             (ainv: TInfo -> History -> MessagePool TMsg -> TState -> Prop) :=
+  Definition TrsAInv (ginv: Inv) (ainv: AInv) :=
     forall ti hst mouts orsout,
       Atomic impl ti hst mouts orsout ->
       forall ist1 ist2,
@@ -47,4 +72,36 @@ Section Impl.
         ainv ti hst mouts ist2.
 
 End Impl.
+
+Lemma trsInv_split:
+  forall impl inv1 inv2,
+    TrsInv impl inv1 ->
+    TrsInv impl inv2 ->
+    TrsInv impl (inv1 /\i inv2).
+Proof.
+  unfold TrsInv, invAnd; intros; dest; split; eauto.
+Qed.
+
+Ltac split_inv := apply trsInv_split.
+
+Lemma trsAInv_split:
+  forall impl ginv ainv1 ainv2,
+    TrsAInv impl ginv ainv1 ->
+    TrsAInv impl ginv ainv2 ->
+    TrsAInv impl ginv (ainv1 /\a ainv2).
+Proof.
+  intros; split; eauto.
+Qed.
+
+Ltac split_ainv := apply trsAInv_split.
+
+Lemma trsAInv_ginv_weaken:
+  forall impl ginv1 ainv,
+    TrsAInv impl ginv1 ainv ->
+    forall ginv2,
+      ginv2 ->i ginv1 ->
+      TrsAInv impl ginv2 ainv.
+Proof.
+  unfold TrsAInv; intros; eauto.
+Qed.
 
